dataplane/Examples/Increment_op_Correctness.thy
@@ -136,7 +136,7 @@ proof (coinduction arbitrary: sg os1 buf os2 rule: wbisim_coinduct_upto'')
         ultimately show ?thesis unfolding R_def by blast
       qed
       moreover have "\<exists>op2'. (step Tau)\<^sup>*\<^sup>* (my_source_op f inc os1 buf os2) op2'
-  \<and> wbisim_cong R (dataflow_op (sg\<lparr>upfro := \<lambda>_. True, pt_tr := change_multiplicities (summ sg) (extract_progress 1 (nxt sg) st) (pt_tr sg)\<rparr>) (map_op (case_sum id id) (case_sum id id) (comp_op [Inr (0, 1) \<mapsto> Inr (1, 1)] buf
+  \<and> wbisim_cong R (dataflow_op (sg\<lparr>pt_tr := change_multiplicities (summ sg) (extract_progress 1 (nxt sg) st) (pt_tr sg)\<rparr>) (map_op (case_sum id id) (case_sum id id) (comp_op [Inr (0, 1) \<mapsto> Inr (1, 1)] buf
     (my_ooo_input_op os1) (my_increment_op inc os2')))) op2'"
         if "invariant f inc os1 buf os2"
           and "(os2', st) = obtain_progress os2"
@@ -144,7 +144,7 @@ proof (coinduction arbitrary: sg os1 buf os2 rule: wbisim_coinduct_upto'')
           and os2' :: "(1, 'b, 'c, 'e) operator_state_scheme"
         using that unfolding R_def invariant_def my_source_op_def obtain_progress_def by (fastforce intro!: wbc_base)
       moreover have "\<exists>op2'. (step Tau)\<^sup>*\<^sup>* (my_source_op f inc os1 buf os2) op2'
-  \<and> wbisim_cong R (dataflow_op (sg\<lparr>upfro := \<lambda>_. True, pt_tr := change_multiplicities (summ sg) (extract_progress 0 (nxt sg) st) (pt_tr sg)\<rparr>) (map_op (case_sum id id) (case_sum id id) (comp_op [Inr (0, 1) \<mapsto> Inr (1, 1)] buf
+  \<and> wbisim_cong R (dataflow_op (sg\<lparr>pt_tr := change_multiplicities (summ sg) (extract_progress 0 (nxt sg) st) (pt_tr sg)\<rparr>) (map_op (case_sum id id) (case_sum id id) (comp_op [Inr (0, 1) \<mapsto> Inr (1, 1)] buf
   (my_ooo_input_op os1') (my_increment_op inc os2)))) op2'"
         if "invariant f inc os1 buf os2"
           and "(os1', st) = obtain_progress os1"
