dataplane/Timely/Propagation_Idempotence.thy
@@ -1,0 +1,35 @@
+theory Propagation_Idempotence
+
+imports
+  Propagation_Exec
+begin
+
+section ‹Idempotence of propagate_all›
+
+text ‹If propagate_all terminates, the resulting configuration has an empty worklist.›
+
+lemma propagate_all_empty_worklist:
+  "propagate_all summary conf = Some conf' ⟹ worklist_is_empty summary conf'"
+  unfolding propagate_all_def
+  by (drule while_option_stop) simp
+
+text ‹On a quiescent configuration, propagate_all is the identity.›
+
+lemma propagate_all_quiescent:
+  "worklist_is_empty summary conf ⟹ propagate_all summary conf = Some conf"
+  unfolding propagate_all_def
+  by (subst while_option_unfold) simp
+
+lemma propagate_all_idem:
+  "propagate_all summary conf = Some conf' ⟹ propagate_all summary conf' = Some conf'"
+  by (rule propagate_all_quiescent[OF propagate_all_empty_worklist])
+
+text ‹Re-propagation does not change the implied frontiers a node reads.›
+
+lemma propagate_all_twice_c_imp:
+  "propagate_all summary conf = Some conf' ⟹
+   propagate_all summary conf' = Some conf'' ⟹
+   c_imp conf'' = c_imp conf'"
+  by (drule propagate_all_idem) simp
+
+end
